update of my work

Dafny/Testworks.py
@@ -1,0 +1,21 @@
+A = [5,4,3,2,1]
+#B = [5,4,3,2,1]
+for i in range(len(A)):
+    for j in range(1,len(A)-i):
+        print("(i,j,len(A) - i,A[j],A[k]) = "+str((i,j,len(A) - i,A[j-1],A[0:j])))
+        if A[j-1] > A[j]:
+            temp = A[j]
+            A[j] = A[j-1]
+            A[j-1] = temp
+# print("-----------")
+# for i in range(len(B)-1,0,-1):
+#     for j in range(0,i):
+#         print((i,j))
+#         if B[j] > B[j+1]:
+#             temp = B[j]
+#             B[j] = B[j+1]
+#             B[j+1] = temp
+
+print("final - ")
+print(A)
+# print(B)
