Dafny/HarrisonAnkers copy.dfy
@@ -1,0 +1,51 @@
+predicate sorted(A: array?<int>, l: int)
+  reads A
+  requires A != null
+  {
+    forall i, j :: 0 <= l <= i <= j < A.Length ==> A[i] <= A[j]
+  }
+  
+predicate partition(A: array?<int>, i: int)
+  reads A
+  requires A != null
+  {
+    forall k, k' :: 0 <= k <= i < k' < A.Length ==> A[k] <= A[k']
+  }
+
+method BubbleSort(A: array?<int>)
+  modifies A
+  requires A != null
+  requires A.Length>0
+  ensures sorted(A, 0)
+  {
+    var i := A.Length - 1;
+    while(i > 0)
+      invariant i < 0 ==> A.Length == 0
+      invariant sorted(A, i)
+      invariant partition(A, i)
+      decreases i
+      {
+        var j := 0;
+        while (j < i)
+          invariant 0 < i < A.Length && 0 <= j <= i
+          invariant sorted(A, i)
+          invariant partition(A, i)
+          invariant forall k :: 0 <= k <= j ==> A[k] <= A[j]
+          decreases i-j
+          {
+            if(A[j] >  A[j+1])
+              {
+                A[j], A[j+1] := A[j+1], A[j];
+              }
+              j := j + 1;
+          }
+          i := i -1;
+      }
+  }
+method Main() {
+  var a := new int[5];
+  a[0], a[1], a[2], a[3], a[4] := 9, 4, 6, 3, 8;
+  BubbleSort(a);
+  var k := 0;
+  while(k < 5) { print a[k], "\n"; k := k+1;}
+}
